Refactoring about Union find.

graph_backup_1/spatial_graph.v
@@ -23,7 +23,7 @@ Proof.
   + exfalso; auto.
 Qed.
 
-Class SpatialGraphSetting: Type := {
+Class PointwiseGraphSetting: Type := {
   Data: Type;
   addr: Type;
   null: addr;
@@ -31,7 +31,7 @@ Class SpatialGraphSetting: Type := {
   addr_eqb: addr -> addr -> bool := fun x y => if addr_eq_dec x y then true else false
 }.
 
-Instance AV_SGraph `{SpatialGraphSetting} : AbsAddr.
+Instance AV_SGraph `{PointwiseGraphSetting} : AbsAddr.
   apply (mkAbsAddr addr (Data * addr * addr) (fun x y => addr_eqb x y)); simpl; intros.
   + unfold addr_eqb.
     destruct (addr_eq_dec p1 p2), (addr_eq_dec p2 p1); try congruence.
@@ -39,12 +39,12 @@ Instance AV_SGraph `{SpatialGraphSetting} : AbsAddr.
     destruct (addr_eq_dec p1 p1); congruence.
 Defined.
 
-Instance AddrDec `{SpatialGraphSetting}: EqDec Addr. apply Build_EqDec. intros. apply (addr_eq_dec t1 t2). Defined.
+Instance AddrDec `{PointwiseGraphSetting}: EqDec Addr. apply Build_EqDec. intros. apply (addr_eq_dec t1 t2). Defined.
 Opaque AddrDec.
 
-Definition Null {SGS: SpatialGraphSetting} : (@Addr AV_SGraph) := null.
+Definition Null {SGS: PointwiseGraphSetting} : (@Addr AV_SGraph) := null.
 
-Class Graph {SGS: SpatialGraphSetting} : Type := {
+Class Graph {SGS: PointwiseGraphSetting} : Type := {
   pg: PreGraph Addr Data;
   bi: BiGraph pg;
   ma: MathGraph pg Null
@@ -56,25 +56,25 @@ Coercion bi : Graph >-> BiGraph.
  
 Coercion ma : Graph >-> MathGraph.
  
-Instance single_graph_double {SGS: SpatialGraphSetting} v d (Hn: v <> Null): Graph := {
+Instance single_graph_double {SGS: PointwiseGraphSetting} v d (Hn: v <> Null): Graph := {
   pg := single_PreGraph _ v d v v;
   bi := single_BiGraph _ v d v v;
   ma := single_MathGraph_double _ _ v d Hn
 }.
  
-Instance single_graph_left {SGS: SpatialGraphSetting} v d (Hn: v <> Null): Graph := {
+Instance single_graph_left {SGS: PointwiseGraphSetting} v d (Hn: v <> Null): Graph := {
   pg := single_PreGraph _ v d v Null;
   bi := single_BiGraph _ v d v Null;
   ma := single_MathGraph_left _ _ v d Hn
 }.
  
-Instance single_graph_right {SGS: SpatialGraphSetting} v d (Hn: v <> Null): Graph := {
+Instance single_graph_right {SGS: PointwiseGraphSetting} v d (Hn: v <> Null): Graph := {
   pg := single_PreGraph _ v d Null v;
   bi := single_BiGraph _ v d Null v;
   ma := single_MathGraph_right _ _ v d Hn
 }.
 
-Class SpatialGraphAssum: Type := {
+Class PointwiseGraphAssum: Type := {
   SGA_Pred: Type;
   SGA_ND: NatDed SGA_Pred;
   SGA_SL : SepLog SGA_Pred;
@@ -85,7 +85,7 @@ Class SpatialGraphAssum: Type := {
   SGA_DSL : DisjointedSepLog SGA_Pred;
   SGA_COSL: CorableOverlapSepLog SGA_Pred;
 
-  SG_Setting: SpatialGraphSetting;
+  SG_Setting: PointwiseGraphSetting;
   trinode : Addr -> Val -> SGA_Pred;
   SGA_MSL: MapstoSepLog AV_SGraph trinode;
   SGA_sMSL: StaticMapstoSepLog AV_SGraph trinode(* ; *)
@@ -98,9 +98,9 @@ Hint Resolve SGA_ND SGA_SL SGA_ClSL SGA_PSL SGA_CoSL SGA_OSL SGA_DSL SGA_COSL SG
 
 Local Open Scope logic.
 
-Section SpatialGraph.
+Section PointwiseGraph.
 
-  Context {SGA : SpatialGraphAssum}.
+  Context {SGA : PointwiseGraphAssum}.
 
   Definition graph_cell (g: Graph) (v : Addr) : SGA_Pred := trinode v (gamma g v).
 
@@ -565,4 +565,4 @@ Instance update_graph (g: Graph) v d l r (Hi: in_math g v l r) (Hn: v <> Null): 
     Implicit Arguments only_two_neighbours [[Vertex] [Data] [EV] [BiGraph]].
   Qed.
 
-End SpatialGraph.
+End PointwiseGraph.
