msl_application/GList_UnionFind.v
@@ -15,92 +15,52 @@ Require Import RamifyCoq.graph.graph_relation.
 Require Import RamifyCoq.graph.subgraph2.
 Require Import RamifyCoq.graph.reachable_computable.
 Require Import RamifyCoq.msl_application.Graph.
+Require Import RamifyCoq.msl_application.UnionFindGraph.
 Require Import RamifyCoq.msl_application.GList.
 
 Local Open Scope logic.
 
 Section GList_UnionFind.
 
-  Context {pSGG: pSpatialGraph_GList}.
-  Context {sSGG: sSpatialGraph_GList nat unit}.
+  Context {pSGG: pPointwiseGraph_GList}.
+  Context {sSGG: sPointwiseGraph_GList nat unit}.
 
-  Local Coercion Graph_LGraph: Graph >-> LGraph.
+  Definition SGraph := (PointwiseGraph addr (addr * unit) (nat * addr) unit).
+
+  Definition LGraph := (@LGraph addr (addr * unit) _ _ nat unit unit).
+  Definition Graph := (@Graph addr (addr * unit) _ _ is_null_SGBA (fun x => (x, tt)) nat unit unit).
+
+  Definition UGraph_LGraph (G: Graph): LGraph := lg_gg G.
+  Definition LGraph_SGraph (G: LGraph): SGraph := Graph_PointwiseGraph G.
+
+  Local Coercion UGraph_LGraph: Graph >-> LGraph.
   Local Coercion LGraph_SGraph: LGraph >-> SGraph.
-  Local Identity Coercion Graph_GeneralGraph: Graph >-> GeneralGraph.
-  Local Identity Coercion LGraph_LabeledGraph: LGraph >-> LabeledGraph.
-  Local Identity Coercion SGraph_SpatialGraph: SGraph >-> SpatialGraph.
+  
+  Local Identity Coercion ULGraph_LGraph: LGraph >-> UnionFindGraph.LGraph.
+  Local Identity Coercion LGraph_LabeledGraph: UnionFindGraph.LGraph >-> LabeledGraph.
   Local Coercion pg_lg: LabeledGraph >-> PreGraph.
-
-  Notation Graph := (@Graph pSGG nat unit unit).
-
-  Lemma uf_root_vgamma: forall (g: Graph) v n, vvalid g v -> vgamma g v = (n, v) -> uf_root g v v.
-  Proof.
-    intros. split.
-    - apply reachable_refl; auto.
-    - intros. apply (parent_loop g _ n); auto.
-  Qed.
-
-  Lemma vgamma_not_dst: forall (g: Graph) x r pa, vgamma g x = (r, pa) -> pa <> x -> dst g (x, tt) = pa.
-  Proof. intros. simpl in H. destruct (SGBA_VE (dst g (x, tt)) null); inversion H; [exfalso |]; auto. Qed.
-
-  Lemma vgamma_not_edge: forall (g: Graph) x r pa, vvalid g x -> vgamma g x = (r, pa) -> pa <> x -> g |= x ~> pa.
-  Proof.
-    intros. assert (vvalid g pa) by (apply valid_parent in H0; auto). hnf. split; [|split]; auto.
-    apply (vgamma_not_dst g x r) in H1; auto. rewrite step_spec. exists (x, tt).
-    pose proof (vvalid_src_evalid _ (liGraph g) _ H). destruct H3. split; auto.
-  Qed.
-
-  Lemma vgamma_not_reachable': forall (g: Graph) x r pa y, vvalid g x -> vgamma g x = (r, pa) -> pa <> x -> reachable g pa y -> ~ reachable g y x.
-  Proof. intros. apply (dst_not_reachable _ (liGraph g) _ pa); auto. apply (vgamma_not_dst g x r); auto. Qed.
-
-  Lemma vgamma_not_reachable: forall (g: Graph) x r pa, vvalid g x -> vgamma g x = (r, pa) -> pa <> x -> ~ reachable g pa x.
-  Proof. intros. assert (vvalid g pa) by (apply valid_parent in H0; auto). apply (vgamma_not_reachable' g x r pa pa); auto. apply reachable_refl; auto. Qed.
-
-  Lemma uf_root_not_eq_root_vgamma: forall (g: Graph) x r pa root, vgamma g x = (r, pa) -> uf_root g x root -> x <> root -> x <> pa.
-  Proof.
-    intros. simpl in H. destruct (SGBA_VE (dst g (x, tt)) null).
-    - hnf in e. destruct H0. apply reachable_ind.reachable_ind in H0. destruct H0. 1: exfalso; auto. destruct H0 as [z [[? [? ?]] [? ?]]]. rewrite step_spec in H4.
-      destruct H4 as [ed [? [? ?]]]. pose proof (conj H7 H4). rewrite (@only_one_edge _ _ _ _ g _ (liGraph g)) in H9; auto. subst ed. rewrite H8 in e.
-      exfalso. apply (@valid_not_null _ _ _ _ g _ (maGraph g)) in H3; auto.
-    - unfold complement, Equivalence.equiv in c. inversion H. clear H H3. assert (vvalid g x) by (destruct H0; apply reachable_head_valid in H; auto).
-      assert (g |= (x, (x, tt) :: nil) is x ~o~> pa satisfying (fun _ => True)). {
-        split; split; intros; hnf; simpl; auto. unfold strong_evalid. assert ((x, tt) = (x, tt)) by auto. rewrite <- (@only_one_edge _ _ _ _ g _ (liGraph g)) in H2; auto.
-        destruct H2. split; [|split]; auto. rewrite H2. split; auto. apply (@valid_graph _ _ _ _ g _ (maGraph g)) in H3. destruct H3 as [_ [? | ?]]; auto.
-        hnf in H3. exfalso; auto.
-      } rewrite H4. intro. rewrite <- H3 in H2. apply (@no_loop_path _ _ _ _ g _ (liGraph g)) in H2. inversion H2.
-  Qed.
-
-  Lemma vgamma_uf_root: forall (g: Graph) x r pa root, vvalid g x -> vgamma g x = (r, pa) -> uf_root g x root -> x <> root -> uf_root g pa root.
-  Proof.
-    intros. pose proof (uf_root_not_eq_root_vgamma g _ _ _ _ H0 H1 H2). destruct H1. split; auto. pose proof (valid_parent g _ _ _ H H0).  
-    assert (Decidable (reachable g pa root)) by (apply Graph_reachable_dec; left; auto). apply decidable_prop_decidable in H6. destruct H6; auto. exfalso.
-    pose proof (lst_out_edge_only_one g (liGraph g) x pa root). simpl in H7. apply H2. apply H7; auto. apply (vgamma_not_dst _ _ r); auto.
-  Qed.
-
-  Instance fml : FML_General addr (addr * unit) nat unit unit LiMaFin (fun x => (x, tt)) is_null_SGBA. Proof. constructor; intros; destruct X; auto. Defined.
+  Local Identity Coercion SGraph_SpatialGraph: SGraph >-> PointwiseGraph.
 
   Global Existing Instance fml.
 
-  Lemma findS_preserves_vgamma: forall (g1 g2: Graph) x r pa, vvalid g1 x -> vgamma g1 x = (r, pa) -> pa <> x -> findS g1 pa g2 -> vgamma g2 x = (r, pa).
-  Proof.
-    intros. assert (Hr: ~ reachable g1 pa x) by (apply vgamma_not_reachable with r; auto). simpl in *. destruct (SGBA_VE (dst g1 (x, tt)) null). 1: inversion H0; exfalso; auto.
-    unfold complement, Equivalence.equiv in c. rewrite <- H0. destruct H2 as [? [[? ?] ?]]. f_equal.
-    - assert (vvalid g2 x) by (rewrite <- H3; auto). specialize (H5 x H H6). unfold Graph_LGraph. rewrite H5. auto.
-    - assert (evalid (predicate_partialgraph (lg_gg g1) (fun n : addr => ~ reachable (lg_gg g1) pa n)) (x, tt)). {
-        simpl. hnf. pose proof (vvalid_src_evalid _ (liGraph g1) _ H). unfold Graph_LGraph in H6. destruct H6. rewrite H6. split; auto.
-      } destruct H2 as [_ [? [_ ?]]]. pose proof H6. rewrite H2 in H8. clear H2. specialize (H7 _ H6 H8). simpl in H7. unfold Graph_LGraph. rewrite <- H7.
-      destruct (SGBA_VE (dst (lg_gg g1) (x, tt)) null); [exfalso |]; auto.
-  Qed.
+  Instance maGraph(G: Graph): MathGraph G is_null_SGBA := maGraph G.
+  Instance finGraph (G: Graph): FiniteGraph G := finGraph G.
+  Instance liGraph (G: Graph):  LstGraph G (fun x => (x, tt)) := liGraph G.
+
+  Definition vgamma := (@vgamma addr (addr * unit) SGBA_VE SGBA_EE is_null_SGBA (fun x => (x, tt)) nat unit unit).
+
+  Definition Graph_gen_redirect_parent (g: Graph) (x: addr) (pa: addr) (H: weak_valid g pa) (Hv: vvalid g x) (Hn: ~ reachable g pa x): Graph :=
+    Graph_gen_redirect_parent g x pa H Hv Hn.
 
   Lemma graph_gen_redirect_parent_ramify: forall (g: Graph) x r pa root (H: weak_valid g root) (Hv: vvalid g x) (Hn: ~ reachable g root x),
-      vgamma g x = (r, pa) -> root <> null ->
-      (vertices_at (vvalid g) g: pred)
+      vgamma g x = (r, pa) -> root <> null -> 
+      (vertices_at (vvalid g) g: pred) 
         |-- vertex_at x (r, pa) * (vertex_at x (r, root) -* vertices_at (vvalid g) (Graph_gen_redirect_parent g x root H Hv Hn)).
   Proof.
     intros. assert (vgamma (Graph_gen_redirect_parent g x root H Hv Hn) x = (r, root)). {
       simpl in *. remember (updateEdgeFunc (dst (lg_gg g)) (x, tt) root (x, tt)).
-      inversion H0. f_equal. unfold updateEdgeFunc in Heqy. destruct (equiv_dec (x, tt) (x, tt)).
-      2: compute in c; exfalso; apply c; auto. subst y. destruct (SGBA_VE root null); [exfalso| ]; auto.
+      inversion H0. unfold vgamma, UnionFindGraph.vgamma. simpl. f_equal. unfold updateEdgeFunc in *. destruct (equiv_dec (x, tt) (x, tt)).
+      2: compute in c; exfalso; apply c; auto. subst y. destruct (SGBA_VE root null); [exfalso| ]; auto. 
     } apply vertices_at_ramif_1; auto. eexists. split; [|split].
     - apply Ensemble_join_Intersection_Complement.
       + unfold Included, In; intro y. intros. subst. auto.
@@ -109,106 +69,17 @@ Section GList_UnionFind.
       + unfold Included, In; intro y. intros. subst. auto.
       + intros; destruct_eq_dec x x0; auto.
     - rewrite vertices_identical_spec. simpl. intros. change (lg_gg g) with (g: LGraph).
-      rewrite Intersection_spec in H3. destruct H3. unfold Complement, In in H4. unfold updateEdgeFunc.
+      rewrite Intersection_spec in H3. destruct H3. unfold Complement, In in H4. unfold vgamma, UnionFindGraph.vgamma. simpl. unfold updateEdgeFunc.
       destruct (equiv_dec (x, tt) (x0, tt)); auto. compute in e. exfalso. inversion e. auto.
   Qed.
 
-  Lemma the_same_root_union: forall (g g1 g2: Graph) x y root,
-      vvalid g x -> vvalid g y -> uf_equiv g g1 -> uf_equiv g1 g2 -> uf_root g1 x root -> uf_root g2 y root -> uf_union g x y g2.
-  Proof. intros. apply (same_root_union g g1 g2 x y root); auto. Qed.
-
-  Lemma uf_equiv_root_the_same: forall (g1 g2: Graph) x root, uf_equiv g1 g2 -> uf_root g1 x root <-> uf_root g2 x root.
-  Proof. intros. pose proof (@uf_equiv_the_same_root _ _ _ _ _ _ _ _ (fun x: addr => (x, tt)) is_null_SGBA fml g1 g2 x root H). apply H0. Qed.
-
-  Lemma uf_equiv_not_reachable: forall (g1 g2: Graph) x r pa root,
-      vvalid g1 x -> vgamma g1 x = (r, pa) -> pa <> x -> uf_equiv g1 g2 -> uf_root g2 pa root -> ~ reachable g2 root x.
-  Proof.
-    intros. pose proof H3. rewrite <- (uf_equiv_root_the_same _ _ pa root H2) in H4. destruct H3. intro. apply H5 in H6. subst x.
-    pose proof (vgamma_not_reachable g1 root r pa H H0 H1). destruct H4. auto.
-  Qed.
-
-  Lemma graph_gen_redirect_parent_equiv': forall (g1 g2: Graph) x root,
-      uf_equiv g1 g2 -> vvalid g2 x -> (~ reachable g2 root x) -> uf_root g2 x root -> uf_equiv g1 (pregraph_gen_dst g2 (x, tt) root).
-  Proof.
-    intros. apply (@uf_equiv_trans _ _ _ _ g2 _ (liGraph g2) _ (maGraph g2) (finGraph g2)); auto. split; intro y; simpl; [intuition |]. intros.
-    assert (Decidable (reachable g2 y x)) by (apply Graph_reachable_dec; left; destruct H3; apply reachable_head_valid in H3; auto).
-    apply decidable_prop_decidable in H5. destruct H5.
-    - pose proof (uf_root_gen_dst_same g2 (liGraph g2) _ _ _ H2 H1 H5). simpl in H6.
-      pose proof (uf_root_unique _ (gen_dst_preserve_lst g2 (liGraph g2) _ _ H1 H0) _ _ _ H4 H6). subst r2.
-      pose proof (uf_root_reachable _ _ _ _ H5 H2). apply (uf_root_unique g2 (liGraph g2) _ _ _ H3 H7).
-    - apply (uf_root_unique _ (gen_dst_preserve_lst g2 (liGraph g2) _ _ H1 H0) y); auto. apply (uf_root_gen_dst_preserve g2 (liGraph g2)); auto.
-  Qed.
-
-  Lemma graph_gen_redirect_parent_equiv: forall (g1 g2: Graph) x r pa root (Hv: vvalid g2 x) (Hn: ~ reachable g2 root x),
-      vvalid g1 x -> vgamma g1 x = (r, pa) -> pa <> x -> uf_equiv g1 g2 -> uf_root g2 pa root -> uf_equiv g1 (pregraph_gen_dst g2 (x, tt) root).
-  Proof.
-    intros. apply graph_gen_redirect_parent_equiv'; auto. rewrite <- (uf_equiv_root_the_same g1); auto.
-    apply (uf_root_edge g1 (liGraph g1) x pa); [| apply (vgamma_not_dst g1 x r) | rewrite (uf_equiv_root_the_same g1 g2)]; auto.
-  Qed.
-
-  Lemma graph_gen_redirect_parent_findS: forall (g1 g2: Graph) x r1 r2 pa pa' (H: weak_valid g2 pa') (Hv: vvalid g2 x) (Hn: ~ reachable g2 pa' x),
-      vvalid g1 x -> vgamma g1 x = (r1, pa) -> pa <> x -> vgamma g2 x = (r2, pa) -> findS g1 pa g2 -> uf_root g2 pa pa' ->
-      findS g1 x (Graph_gen_redirect_parent g2 x pa' H Hv Hn).
-  Proof.
-    intros. hnf. simpl. destruct H4 as [? [? ?]]. hnf in H4. simpl in H4. unfold predicate_vvalid, predicate_weak_evalid in H4. split; [|split].
-    - assert (forall v, ~ reachable (lg_gg g1) x v -> ~ reachable (lg_gg g1) pa v). {
-        intros. intro. apply H8. pose proof (gamma_parent_reachable_included g1 x r1 pa H0 H1). apply H10. auto. }
-      assert (forall v, ~ reachable (lg_gg g1) pa v <-> ~ reachable (lg_gg g1) x v \/ x = v). {
-        intros. split; intros.
-        - destruct_eq_dec x v; [right | left]; auto. intro. apply H9. apply reachable_ind.reachable_ind in H11. destruct H11. 1: exfalso; auto.
-          destruct H11 as [z [[_ [_ ?]] [? ?]]]. rewrite (dst_step g1 (liGraph g1) x pa) in H11; auto; [subst pa | apply (vgamma_not_dst g1 x r1)]; auto.
-        - destruct H9.
-          + apply H8; auto.
-          + subst v. apply vgamma_not_reachable with r1; auto.
-      } hnf. simpl. unfold predicate_vvalid, predicate_weak_evalid. simpl. destruct H4 as [? [? [? ?]]]. split; [|split; [|split]]; intros.
-      + split; intros; destruct H13; split; auto; apply H8 in H14; pose proof (conj H13 H14); [rewrite H4 in H15 | rewrite <- H4 in H15]; destruct H15; auto.
-      + split; intros; destruct H13.
-        * pose proof (H8 _ H14). pose proof (conj H13 H15). rewrite H10 in H16. destruct H16. rewrite H9 in H17. destruct H17. 1: split; auto. symmetry in H17.
-          pose proof (conj H17 H16). rewrite (@only_one_edge _ _ _ _ g2 _ (liGraph g2)) in H18; auto. subst e. pose proof (vvalid_src_evalid _ (liGraph g1) _ H0).
-          destruct H18 as [? _]. unfold Graph_LGraph in H18. rewrite H18 in H14. exfalso. apply H14. apply reachable_refl. auto.
-        * pose proof (H8 _ H14). pose proof (conj H13 H15). rewrite <- H10 in H16. destruct H16. rewrite H9 in H17. destruct H17. 1: split; auto. symmetry in H17.
-          pose proof (conj H17 H16). rewrite (@only_one_edge _ _ _ _ g1 _ (liGraph g1)) in H18; auto. subst e. pose proof (vvalid_src_evalid _ (liGraph g2) _ Hv).
-          destruct H18 as [? _]. unfold Graph_LGraph in H18. rewrite H18 in H14. exfalso. apply H14. apply reachable_refl. auto.
-      + destruct H13, H14. apply H8 in H15. apply H8 in H16. apply H11; auto.
-      + unfold updateEdgeFunc. destruct (equiv_dec (x, tt) e).
-        * unfold Equivalence.equiv in e0. subst e. pose proof (vvalid_src_evalid _ (liGraph g1) _ H0).
-          destruct H15. unfold Graph_LGraph in H15. destruct H13. exfalso. apply H17. rewrite H15. apply reachable_refl; auto.
-        * destruct H13, H14. apply H8 in H15. apply H8 in H16. apply H12; auto.
-    - apply (graph_gen_redirect_parent_equiv _ _ _ r1 pa); auto.
-    - apply H7.
-  Qed.
-
-  Lemma diff_root_union_1: forall (g g1 g2: Graph) x y x_root y_root,
-      uf_equiv g g1 -> uf_root g1 x x_root -> uf_equiv g1 g2 -> uf_root g2 y y_root -> x_root <> y_root ->
-      (@weak_valid _ _ _ _ g2 _ (maGraph g2) y_root) -> vvalid g2 x_root ->
-      ~ reachable g2 y_root x_root -> uf_union g x y (pregraph_gen_dst g2 (x_root, tt) y_root).
-  Proof.
-    intros. assert (uf_equiv g g2) by (apply (@uf_equiv_trans _ _ _ _ g1 _ (liGraph g1) _ (maGraph g1) (finGraph g1)); auto).
-    pose proof (uf_equiv_union g g2 (Graph_gen_redirect_parent g2 x_root y_root H4 H5 H6) x y H7). simpl in H8. apply H8.
-    apply (@diff_root_union _ _ _ _ _ _ _ _ (fun x: addr => (x, tt)) is_null_SGBA fml); auto. apply (uf_equiv_root_the_same g1); auto.
-  Qed.
-
-  Lemma diff_root_union_2: forall (g g1 g2: Graph) x y x_root y_root,
-      uf_equiv g g1 -> uf_root g1 x x_root -> uf_equiv g1 g2 -> uf_root g2 y y_root -> x_root <> y_root -> (@weak_valid _ _ _ _ g2 _ (maGraph g2) x_root) -> vvalid g2 y_root ->
-      ~ reachable g2 x_root y_root -> uf_union g x y (pregraph_gen_dst g2 (y_root, tt) x_root).
-  Proof.
-    intros. assert (uf_equiv g g2) by (apply (@uf_equiv_trans _ _ _ _ g1 _ (liGraph g1) _ (maGraph g1) (finGraph g1)); auto).
-    pose proof (uf_equiv_union g g2 (Graph_gen_redirect_parent g2 y_root x_root H4 H5 H6) y x H7). simpl in H8. apply uf_union_sym. apply H8.
-    apply (@diff_root_union _ _ _ _ _ _ _ _ (fun x: addr => (x, tt)) is_null_SGBA fml); auto. apply (uf_equiv_root_the_same g1); auto.
-  Qed.
-
-  Lemma graph_gen_redirect_parent_vgamma: forall (g1 g2: Graph) x r pa y (H: weak_valid g1 x) (Hv: vvalid g1 y) (Hn: ~ reachable g1 x y),
-      vgamma g1 x = (r, pa) -> g2 = (Graph_gen_redirect_parent g1 y x H Hv Hn) -> vgamma g2 x = (r, pa).
-  Proof.
-    intros. rewrite H1. clear H1. simpl in *. inversion H0. f_equal. unfold updateEdgeFunc.
-    destruct (equiv_dec (y, tt) (x, tt)); [hnf in e; inversion e; subst; exfalso; apply Hn; apply reachable_refl|]; auto.
-  Qed.
+  Definition Graph_vgen (G: Graph) (x: addr) (d: nat) : Graph := Graph_vgen G x d.
 
   Lemma graph_vgen_ramify: forall (g: Graph) x r1 r2 pa,
       vvalid g x -> vgamma g x = (r1, pa) -> (vertices_at (vvalid g) g: pred) |-- vertex_at x (r1, pa) * (vertex_at x (r2, pa) -* vertices_at (vvalid g) (Graph_vgen g x r2)).
   Proof.
     intros. assert (vgamma (Graph_vgen g x r2) x = (r2, pa)). {
-      simpl in *. inversion H0. f_equal. unfold update_vlabel. destruct (equiv_dec x x); auto. compute in c. exfalso; auto.
+      simpl in *. inversion H0. unfold vgamma, UnionFindGraph.vgamma. simpl. f_equal. unfold update_vlabel. destruct (equiv_dec x x); auto. compute in c. exfalso; auto.
     } apply vertices_at_ramif_1; auto. eexists. split; [|split].
     - apply Ensemble_join_Intersection_Complement.
       + unfold Included, In; intro y. intros. subst. auto.
@@ -217,7 +88,8 @@ Section GList_UnionFind.
       + unfold Included, In; intro y. intros. subst. auto.
       + intros; destruct_eq_dec x x0; auto.
     - rewrite vertices_identical_spec. simpl. intros. change (lg_gg g) with (g: LGraph).
-      rewrite Intersection_spec in H2. destruct H2. unfold Complement, In in H3. unfold update_vlabel. f_equal. destruct (equiv_dec x x0); auto. hnf in e. exfalso; auto.
+      rewrite Intersection_spec in H2. destruct H2. unfold Complement, In in H3. unfold vgamma, UnionFindGraph.vgamma. simpl.
+      unfold update_vlabel. f_equal. destruct (equiv_dec x x0); auto. hnf in e. exfalso; auto.
   Qed.
 
   Lemma uf_under_bound_redirect_parent: forall (g: Graph) root x (Hw : weak_valid g root) (Hv : vvalid g x) (Hr: ~ reachable g root x),
@@ -237,7 +109,7 @@ Section GList_UnionFind.
     intros. hnf in H1 |-* . simpl. unfold uf_bound, id in *. intros. destruct p as [p l]. destruct (redirect_to_root g (liGraph g) _ _ _ _ _ Hv Hr H0 H3 H4).
     - destruct H5; apply H1; auto.
     - destruct H5 as [? [l1 [? ?]]]. subst l. subst v. simpl. destruct H7 as [[_ ?] [? _]]. specialize (H1 _ Hv _ H6 H5). simpl in H1. rewrite app_length. simpl.
-      clear - H H1. unfold Graph_LGraph in H. intuition.
+      clear - H H1. unfold Graph_LGraph in H. assert (vlabel (lg_gg g) x < vlabel (lg_gg g) root) by intuition. intuition.
   Qed.
 
   Lemma uf_under_bound_redirect_parent_eq: forall (g: Graph) root x (Hw : weak_valid g root) (Hv : vvalid g x) (Hr: ~ reachable g root x),
@@ -247,7 +119,8 @@ Section GList_UnionFind.
     intros. hnf in H1 |-* . simpl. unfold uf_bound, id, update_vlabel in *. intros. destruct p as [p l]. destruct (redirect_to_root g (liGraph g) _ _ _ _ _ Hv Hr H0 H3 H4).
     - destruct H5. specialize (H1 _ H2 _ H5 H6). simpl in H1 |-* . clear -H1. destruct (equiv_dec root v); [hnf in e; subst v |]; intuition.
     - destruct H5 as [? [l1 [? ?]]]. subst l. subst v. destruct (equiv_dec root root). 2: compute in c; exfalso; apply c; auto. simpl. destruct H7 as [[_ ?] [? _]].
-      specialize (H1 _ Hv _ H6 H5). simpl in H1. rewrite app_length. simpl. clear -H H1. unfold Graph_LGraph in *. intuition.
+      specialize (H1 _ Hv _ H6 H5). simpl in H1. rewrite app_length. simpl. clear -H H1. unfold Graph_LGraph in *. assert (vlabel (lg_gg g) x = vlabel g root) by intuition. intuition.
   Qed.
 
+  Definition make_set_Graph (default_dv: nat) (default_de: unit) (default_dg: unit) (v: addr) (g: Graph) (Hn: v <> null) (Hi: ~ vvalid g v) : Graph := make_set_Graph default_dv default_de default_dg v g Hn Hi.
 End GList_UnionFind.
