sample_mark/verif_dispose_bi.v
@@ -22,7 +22,7 @@ Local Coercion Graph_LGraph: Graph >-> LGraph.
 Local Coercion LGraph_SGraph: LGraph >-> SGraph.
 Local Identity Coercion Graph_GeneralGraph: Graph >-> GeneralGraph.
 Local Identity Coercion LGraph_LabeledGraph: LGraph >-> LabeledGraph.
-Local Identity Coercion SGraph_SpatialGraph: SGraph >-> SpatialGraph.
+Local Identity Coercion SGraph_PointwiseGraph: SGraph >-> PointwiseGraph.
 Local Coercion pg_lg: LabeledGraph >-> PreGraph.
 
 Notation vertices_at sh g P := (@vertices_at _ _ _ _ _ _ (@SGP pSGG_VST bool unit (sSGG_VST sh)) _ g P).
